DT and RF made modular

ocaml/lib/DT.ml
@@ -1,15 +1,43 @@
+open Equalities
 open Features
 open Utils
+open Xp
 
-type 'class0 decisionTree =
-| Leaf of 'class0
-| Node of fin * testIndex * 'class0 decisionTree * 'class0 decisionTree
+module DT =
+ functor (F:FeatureSig) ->
+ functor (K':UsualDecidableType) ->
+ struct
+  module K = K'
 
-(** val evalDT :
-    int -> featureSig -> 'a1 decisionTree -> featureVec -> 'a1 **)
+  type t_ =
+  | Leaf of K.t
+  | Node of fin * testIndex * t_ * t_
 
-let rec evalDT n fs dt x =
-  match dt with
-  | Leaf c -> c
-  | Node (i, t, dt1, dt2) ->
-    if featureTest' n fs x i t then evalDT n fs dt1 x else evalDT n fs dt2 x
+  (** val t__rect :
+      (K.t -> 'a1) -> (fin -> testIndex -> t_ -> 'a1 -> t_ -> 'a1 -> 'a1) ->
+      t_ -> 'a1 **)
+
+  let rec t__rect f f0 = function
+  | Leaf c -> f c
+  | Node (i, t1, dt1, dt2) ->
+    f0 i t1 dt1 (t__rect f f0 dt1) dt2 (t__rect f f0 dt2)
+
+  (** val t__rec :
+      (K.t -> 'a1) -> (fin -> testIndex -> t_ -> 'a1 -> t_ -> 'a1 -> 'a1) ->
+      t_ -> 'a1 **)
+
+  let rec t__rec f f0 = function
+  | Leaf c -> f c
+  | Node (i, t1, dt1, dt2) ->
+    f0 i t1 dt1 (t__rec f f0 dt1) dt2 (t__rec f f0 dt2)
+
+  type t = t_
+
+  (** val eval : t -> featureVec -> K.t **)
+
+  let rec eval dt x =
+    match dt with
+    | Leaf c -> c
+    | Node (i, t0, dt1, dt2) ->
+      if featureTest' F.n F.fs x i t0 then eval dt1 x else eval dt2 x
+ end
