ocaml/lib/DT.mli
@@ -1,8 +1,32 @@
+open Equalities
 open Features
 open Utils
+open Xp
 
-type 'class0 decisionTree =
-| Leaf of 'class0
-| Node of fin * testIndex * 'class0 decisionTree * 'class0 decisionTree
+module DT :
+ functor (F:FeatureSig) ->
+ functor (K':UsualDecidableType) ->
+ sig
+  module K :
+   sig
+    type t = K'.t
 
-val evalDT : int -> featureSig -> 'a1 decisionTree -> featureVec -> 'a1
+    val eq_dec : t -> t -> bool
+   end
+
+  type t_ =
+  | Leaf of K.t
+  | Node of fin * testIndex * t_ * t_
+
+  val t__rect :
+    (K.t -> 'a1) -> (fin -> testIndex -> t_ -> 'a1 -> t_ -> 'a1 -> 'a1) -> t_
+    -> 'a1
+
+  val t__rec :
+    (K.t -> 'a1) -> (fin -> testIndex -> t_ -> 'a1 -> t_ -> 'a1 -> 'a1) -> t_
+    -> 'a1
+
+  type t = t_
+
+  val eval : t -> featureVec -> K.t
+ end
