ocaml/lib/RF.mli
@@ -1,17 +1,60 @@
-open DT
+open Datatypes
 open Features
 open List0
+open Orders
 open Utils
+open Xp
 
-module StringVoting :
+module RF :
+ functor (F:FeatureSig) ->
+ functor (K':UsualOrderedType) ->
  sig
-  val vote : string -> string list -> string
+  module K :
+   sig
+    type t = K'.t
 
-  val count_occ : string list -> string -> int
+    val compare : t -> t -> comparison
+
+    val eq_dec : t -> t -> bool
+   end
+
+  module KFull :
+   UsualOrderedTypeFull with type t = K.t
+
+  module KVoting :
+   sig
+    val vote : K.t -> K.t list -> K.t
+
+    val count_occ : K.t list -> K.t -> int
+   end
+
+  module Dt :
+   sig
+    module K :
+     sig
+      type t = K'.t
+
+      val eq_dec : K'.t -> K'.t -> bool
+     end
+
+    type t_ =
+    | Leaf of K'.t
+    | Node of fin * testIndex * t_ * t_
+
+    val t__rect :
+      (K'.t -> 'a1) -> (fin -> testIndex -> t_ -> 'a1 -> t_ -> 'a1 -> 'a1) ->
+      t_ -> 'a1
+
+    val t__rec :
+      (K'.t -> 'a1) -> (fin -> testIndex -> t_ -> 'a1 -> t_ -> 'a1 -> 'a1) ->
+      t_ -> 'a1
+
+    type t = t_
+
+    val eval : t -> featureVec -> K'.t
+   end
+
+  type t = Dt.t nelist
+
+  val eval : t -> featureVec -> K.t
  end
-
-type coq_class = string
-
-type randomForest = coq_class decisionTree nelist
-
-val evalRF : int -> featureSig -> randomForest -> featureVec -> coq_class
