coq/Extract.v
@@ -1,11 +1,14 @@
 Require Extraction ExtrOcamlBasic ExtrOcamlNatInt ExtrOcamlZInt ExtrOCamlFloats ExtrOcamlNativeString.
 Require List.
 
-From RFXP Require Import Utils Features Explainer.
+From RFXP Require Import Utils Features DT RF.
 
 Set Extraction Output Directory "../ocaml/lib".
 
 Extraction Blacklist List String.
 
 Extraction Language OCaml.
-Separate Extraction Main boolean_feature float_feature string_enum_feature enum_feature to_nat to_fin'.
+Separate Extraction
+    to_nat to_fin'
+    boolean_feature float_feature string_enum_feature enum_feature
+    DT RF.
